test.lean
@@ -5,6 +5,7 @@
 
 
 import Tests.TestMain
+import Tests.TestComplexity
 import LeanC.Arrays
 
 open Lean IO
@@ -23,4 +24,4 @@ def runAll (runners : List (IO UInt32)) : IO UInt32 := do
 def main : IO UInt32 := do
   -- Add each test module's `main` here in the same order as imports above.
   -- Expand this list when new tests are added under `tests/`.
-  runAll [TestMain.test]
+  runAll [TestMain.test, TestComplexity.test]
